Code/Syntax/Signature.v
@@ -4,3 +4,52 @@ Require Export Syntax.Signature.Terms.
 Require Export Syntax.Signature.TermWeakenings.
 Require Export Syntax.Signature.TermSubstitutions.
 Require Export Syntax.Signature.RewritingSystem.
+
+Record AFS (B : Type) (F : Type) (R : Type) :=
+  {
+    Arity : F -> Ty B ;
+    Vars : R -> Con B ;
+    Tars : R -> B ;
+    Lhs : forall (r : R), Tm Arity (Vars r) (Base (Tars r)) ;
+    Rhs : forall (r : R), Tm Arity (Vars r) (Base (Tars r))
+  }.
+
+Arguments Arity {_ _ _}.
+Arguments Vars {_ _ _}.
+Arguments Tars {_ _ _}.
+Arguments Lhs {_ _ _}.
+Arguments Rhs {_ _ _}.
+
+Module AFSNotation.
+  Definition Tm
+             {B : Type}
+             {F : Type}
+             {R : Type}
+             (X : AFS B F R)
+             (C : Con B)
+             (A : Ty B)
+  : Type
+    := Terms.Tm (Arity X) C A.
+
+  Definition BetaRed
+             {B : Type}
+             {F : Type}
+             {R : Type}
+             (X : AFS B F R)
+             {C : Con B}
+             {A : Ty B}
+             (t1 t2 : Tm X C A)
+    : Prop
+    := RewritingSystem.BetaRed t1 t2.
+
+  Definition Rew
+             {B : Type}
+             {F : Type}
+             {R : Type}
+             (X : AFS B F R)
+             {C : Con B}
+             {A : Ty B}
+             (t1 t2 : Tm X C A)
+    : Prop
+    := RewritingSystem.Rew (Lhs X) (Rhs X) t1 t2.
+End AFSNotation.
