Code/Syntax/Signature/RewritingSystem.v
@@ -4,42 +4,126 @@ Require Import Syntax.Signature.Terms.
 Require Import Syntax.Signature.TermWeakenings.
 Require Import Syntax.Signature.TermSubstitutions.
 
+(*
 Inductive Rew
           {B : Type}
           {F : Type}
           {ar : F -> Ty B}
           {R : Type}
           {Rcon : R -> Con B}
-          {Rtar : R -> Ty B}
-  : forall (lhs rhs : forall (r : R), Tm ar (Rcon r) (Rtar r))
+          {Rtar : R -> B}
+  : forall (lhs rhs : forall (r : R), Tm ar (Rcon r) (Base (Rtar r)))
            {C : Con B}
            {A : Ty B},
     Tm ar C A -> Tm ar C A -> Type
   :=
-| Trans : forall {lhs rhs : forall (r : R), Tm ar (Rcon r) (Rtar r)}
+| Trans : forall {lhs rhs : forall (r : R), Tm ar (Rcon r) (Base (Rtar r))}
                  {C : Con B}
                  {A : Ty B}
                  {t1 t2 t3 : Tm ar C A},
     Rew lhs rhs t1 t2 -> Rew lhs rhs t2 t3 -> Rew lhs rhs t1 t3
-| Rew_App_l : forall {lhs rhs : forall (r : R), Tm ar (Rcon r) (Rtar r)}
+| Rew_App_l : forall {lhs rhs : forall (r : R), Tm ar (Rcon r) (Base (Rtar r))}
                      {C : Con B}
                      {A B : Ty B}
                      {f1 f2 : Tm ar C (A ⟶ B)}
                      (x : Tm ar C A),
     Rew lhs rhs f1 f2 -> Rew lhs rhs (f1 · x) (f2 · x)
-| Rew_App_r : forall {lhs rhs : forall (r : R), Tm ar (Rcon r) (Rtar r)}
+| Rew_App_r : forall {lhs rhs : forall (r : R), Tm ar (Rcon r) (Base (Rtar r))}
                      {C : Con B}
                      {A B : Ty B}
                      (f : Tm ar C (A ⟶ B))
                      {x1 x2 : Tm ar C A},
     Rew lhs rhs x1 x2 -> Rew lhs rhs (f · x1) (f · x2)
-| Rew_Lam : forall {lhs rhs : forall (r : R), Tm ar (Rcon r) (Rtar r)}
+| Rew_Lam : forall {lhs rhs : forall (r : R), Tm ar (Rcon r) (Base (Rtar r))}
                    {C : Con B}
                    {A B : Ty B}
                    {f1 f2 : Tm ar (A ,, C) B},
     Rew lhs rhs f1 f2 -> Rew lhs rhs (λ f1) (λ f2)
-| BaseRew : forall {lhs rhs : forall (r : R), Tm ar (Rcon r) (Rtar r)}
+| BaseRew : forall {lhs rhs : forall (r : R), Tm ar (Rcon r) (Base (Rtar r))}
                    {C : Con B}
                    (r : R)
                    (s : Sub ar C (Rcon r)),
     Rew lhs rhs (subTm (lhs r) s) (subTm (rhs r) s).
+ *)
+
+Definition beta_sub
+           {B : Type}
+           {F : Type}
+           {ar : F -> Ty B}
+           {C : Con B}
+           {A : Ty B}
+           (t : Tm ar C A)
+  : Sub ar C (A ,, C)
+  := ExtendSub (idSub C ar) t.
+
+Inductive BetaRed
+          {B : Type}
+          {F : Type}
+          {ar : F -> Ty B}
+          {C : Con B}
+  : forall {A : Ty B}, Tm ar C A -> Tm ar C A -> Prop
+  :=
+| BetaTrans : forall {A : Ty B}
+                     {t1 t2 t3 : Tm ar C A},
+    BetaRed t1 t2 -> BetaRed t2 t3 -> BetaRed t1 t3
+| BetaRew_App_l : forall {A1 A2 : Ty B}
+                         {f1 f2 : Tm ar C (A1 ⟶ A2)}
+                         (x : Tm ar C A1),
+    BetaRed f1 f2 -> BetaRed (f1 · x) (f2 · x)
+| BetaRew_App_r : forall {A1 A2 : Ty B}
+                         (f : Tm ar C (A1 ⟶ A2))
+                         {x1 x2 : Tm ar C A1},
+    BetaRed x1 x2 -> BetaRed (f · x1) (f · x2)
+| BetaRew_Lam : forall {A1 A2 : Ty B}
+                       {f1 f2 : Tm ar (A1 ,, C) A2},
+    BetaRed f1 f2 -> BetaRed (λ f1) (λ f2)
+| BetaBeta : forall {A1 A2 : Ty B}
+                    (f : Tm ar (A1 ,, C) A2)
+                    (x : Tm ar C A1),
+    BetaRed ((λ f) · x) (subTm f (beta_sub x)).
+
+Arguments BetaTrans {_ _ _ _} {_ _ _ _} _ _.
+Arguments BetaRew_App_l {_ _ _ _} {_ _ _ _} _ _.
+Arguments BetaRew_App_r {_ _ _ _} {_ _} _ {_ _} _.
+Arguments BetaRew_Lam {_ _ _ _} {_ _ _ _} _.
+Arguments BetaBeta {_ _ _ _} {_ _} _ _.
+
+Inductive Rew
+          {B : Type}
+          {F : Type}
+          {ar : F -> Ty B}
+          {R : Type}
+          {Rcon : R -> Con B}
+          {Rtar : R -> B}
+          (lhs rhs : forall (r : R), Tm ar (Rcon r) (Base (Rtar r)))
+          {C : Con B}
+  : forall {A : Ty B}, Tm ar C A -> Tm ar C A -> Prop
+  :=
+| Trans : forall {A : Ty B}
+                 {t1 t2 t3 : Tm ar C A},
+    Rew lhs rhs t1 t2 -> Rew lhs rhs t2 t3 -> Rew lhs rhs t1 t3
+| Rew_App_l : forall {A1 A2 : Ty B}
+                     {f1 f2 : Tm ar C (A1 ⟶ A2)}
+                     (x : Tm ar C A1),
+    Rew lhs rhs f1 f2 -> Rew lhs rhs (f1 · x) (f2 · x)
+| Rew_App_r : forall {A1 A2 : Ty B}
+                     (f : Tm ar C (A1 ⟶ A2))
+                     {x1 x2 : Tm ar C A1},
+    Rew lhs rhs x1 x2 -> Rew lhs rhs (f · x1) (f · x2)
+| Rew_Lam : forall {A1 A2 : Ty B}
+                   {f1 f2 : Tm ar (A1 ,, C) A2},
+    Rew lhs rhs f1 f2 -> Rew lhs rhs (λ f1) (λ f2)
+| Beta : forall {A1 A2 : Ty B}
+                (f : Tm ar (A1 ,, C) A2)
+                (x : Tm ar C A1),
+    Rew lhs rhs ((λ f) · x) (subTm f (beta_sub x))
+| BaseRew : forall (r : R)
+                   (s : Sub ar C (Rcon r)),
+    Rew lhs rhs (subTm (lhs r) s) (subTm (rhs r) s).
+
+Arguments Trans {_ _ _ _ _ _ _ _ _} {_ _ _ _} _ _.
+Arguments Rew_App_l {_ _ _ _ _ _ _ _ _} {_ _ _ _} _ _.
+Arguments Rew_App_r {_ _ _ _ _ _ _ _ _} {_ _} _ {_ _} _.
+Arguments Rew_Lam {_ _ _ _ _ _ _ _ _} {_ _ _ _} _.
+Arguments Beta {_ _ _ _ _ _ _ _ _} {_ _} _ _.
+Arguments BaseRew {_ _ _ _ _ _ _ _ _} _ _.
