Code/Syntax/Signature/TermSubstitutions.v
@@ -15,12 +15,12 @@ Fixpoint dropSub
          {C1 C2 : Con B}
          {F : Type}
          {ar : F -> Ty B}
-         {A : Ty B}
+         (A : Ty B)
          (s : Sub ar C1 C2)
   : Sub ar (A ,, C1) C2
   := match s with
      | ToEmpty _ => ToEmpty _
-     | s & t => dropSub s & wkTm t (Drop A (idWk _))
+     | s & t => dropSub A s & wkTm t (Drop A (idWk _))
      end.
 
 Definition keepSub
@@ -28,10 +28,35 @@ Definition keepSub
            {C1 C2 : Con B}
            {F : Type}
            {ar : F -> Ty B}
-           {A : Ty B}
+           (A : Ty B)
            (s : Sub ar C1 C2)
   : Sub ar (A ,, C1) (A ,, C2)
-  := dropSub s & TmVar Vz.
+  := dropSub A s & TmVar Vz.
+
+Fixpoint idSub
+         {B : Type}
+         (C : Con B)
+         {F : Type}
+         (ar : F -> Ty B)
+         {struct C}
+  : Sub ar C C
+  := match C with
+     | ∙ => ToEmpty _
+     | A ,, C => dropSub A (idSub C ar) & TmVar Vz
+     end.
+
+Fixpoint wkToSub
+         {B : Type}
+         {C1 C2 : Con B}
+         {F : Type}
+         {ar : F -> Ty B}
+         (w : Wk C1 C2)
+  : Sub ar C1 C2
+  := match w with
+     | EmptyWk => ToEmpty ∙
+     | Keep A w => keepSub A (wkToSub w)
+     | Drop A w => dropSub A (wkToSub w)
+     end.
 
 Definition subVar
            {B : Type}
@@ -64,6 +89,252 @@ Fixpoint subTm
   := match t with
      | BaseTm f => fun _ _ => BaseTm f
      | TmVar v => fun _ s => subVar v s
-     | Lam f => fun _ s => Lam (subTm f (keepSub s))
+     | Lam f => fun _ s => Lam (subTm f (keepSub _ s))
      | App f t => fun _ s => App (subTm f s) (subTm t s) 
      end.
+
+Definition compSub
+           {B : Type}
+           {C1 C2 C3 : Con B}
+           {F : Type}
+           {ar : F -> Ty B}
+           (s2 : Sub ar C2 C3)
+           (s1 : Sub ar C1 C2)
+  : Sub ar C1 C3.
+Proof.
+  induction s2 as [ | ? ? ? ? s2 IHs2 t ].
+  - apply ToEmpty.
+  - exact (IHs2 s1 & subTm t s1).
+Defined.
+
+(** LEMMATA ON SUBSTITUTION *)
+Require Import Coq.Program.Equality.
+
+Definition wkToSub_id
+           {B : Type}
+           {C : Con B}
+           {F : Type}
+           {ar : F -> Ty B}
+  : wkToSub (idWk C) = idSub C ar.
+Proof.
+  induction C as [ | A C IHC ].
+  - reflexivity.
+  - simpl.
+    rewrite IHC.
+    reflexivity.
+Qed.
+
+Definition wkVar_is_subVar
+           {B : Type}
+           {C2 : Con B}
+           {A : Ty B}
+           {F : Type}
+           {ar : F -> Ty B}
+           (v : Var C2 A)
+           {C1 : Con B}
+           (w : Wk C1 C2)
+  : @TmVar B F ar _ _ (wkVar v w) = subVar v (wkToSub w).
+Proof.
+  (*
+  induction w.
+  - inversion v.
+  - inversion v ; subst.
+    + admit.
+    + admit.
+  - simpl.
+    specialize (IHw v).
+    inversion v ; subst.
+    + simpl.
+      cbn.
+      specialize (IHw v).
+      admit.
+    +  simpl.
+      rewrite <- 
+      rewrite IHw.
+      rewrite <- IHw.
+      simpl.
+      cbn.
+  induction v.
+  - dependent induction w.
+    + reflexivity.
+    + simpl.
+      specialize (IHw ar _ _ w eq_refl).
+      Locate "~=".
+      simpl.
+      admit.
+  -*)
+Admitted.
+    
+Proposition wkTm_is_subTm
+            {B : Type}
+            {C2 : Con B}
+            {A : Ty B}
+            {F : Type}
+            {ar : F -> Ty B}
+            (t : Tm ar C2 A)
+            {C1 : Con B}
+            (w : Wk C1 C2)
+  : wkTm t w = subTm t (wkToSub w).
+Proof.
+  revert w.
+  revert C1.
+  induction t ; intros C1 w ; simpl.
+  - reflexivity.
+  - apply wkVar_is_subVar.
+  - simpl.
+    rewrite IHt.
+    reflexivity.
+  - simpl.
+    rewrite IHt1.
+    rewrite IHt2.
+    reflexivity.
+Qed.
+
+Proposition subTm_comp
+            {B : Type}
+            {C3 : Con B}
+            {A : Ty B}
+            {F : Type}
+            {ar : F -> Ty B}
+            (t : Tm ar C3 A)
+            {C1 C2 : Con B}
+            (s1 : Sub ar C1 C2)
+            (s2 : Sub ar C2 C3)
+  : subTm (subTm t s2) s1 = subTm t (compSub s2 s1).
+Proof.
+  revert s2 s1.
+  revert C1 C2.
+  induction t ; simpl ; intros C1 C2 s1 s2.
+  - reflexivity.
+  - admit.
+  - rewrite IHt.
+    (*
+    rewrite comp_keepSub.
+    reflexivity.
+     *)
+    admit.
+  - rewrite IHt1, IHt2.
+    reflexivity.
+Admitted.
+
+
+Proposition comp_keepSub
+            {B : Type}
+            {C1 C2 C3 : Con B}
+            {F : Type}
+            {ar : F -> Ty B}
+            {A : Ty B}
+            (s1 : Sub ar C1 C2)
+            (s2 : Sub ar C2 C3)
+  : compSub (keepSub A s2) (keepSub A s1)
+    =
+    keepSub A (compSub s2 s1).
+Proof.
+  unfold keepSub.
+  simpl.
+  cbn.
+  f_equal.
+  induction s2.
+  - reflexivity.
+  - simpl.
+    rewrite IHs2 ; clear IHs2.
+    f_equal.
+    rewrite !wkTm_is_subTm.
+    rewrite !subTm_comp.
+    f_equal.
+    simpl ; cbn.
+    rewrite !wkToSub_id.
+    clear t s2 A0 C2.
+Admitted.
+
+Proposition subVar_id
+            {B : Type}
+            {C : Con B}
+            {A : Ty B}
+            {F : Type}
+            {ar : F -> Ty B}
+            (v : Var C A)
+  : subVar v (idSub C ar) = TmVar v.
+Proof.
+  induction v.
+  - reflexivity.
+  - simpl ; cbn.
+    admit.
+Admitted.
+
+Proposition Sub_id_left
+            {B : Type}
+            {C1 C2 : Con B}
+            {F : Type}
+            {ar : F -> Ty B}
+            (s : Sub ar C1 C2)
+  : compSub (idSub _ _) s = s.
+Proof.
+  revert s.
+  revert C1.
+  induction C2 ; intros C1 s.
+  - cbn.
+    dependent induction s.
+    reflexivity.
+  - simpl.
+Admitted.
+
+Proposition Sub_id_right
+            {B : Type}
+            {C1 C2 : Con B}
+            {F : Type}
+            {ar : F -> Ty B}
+            (s : Sub ar C1 C2)
+  : compSub s (idSub _ _) = s.
+Proof.
+  induction s.
+  - reflexivity.
+  - simpl ; cbn.
+    rewrite IHs.
+    
+Admitted.
+
+Proposition keep_drop
+            {B : Type}
+            {C1 C2 : Con B}
+            {A : Ty B}
+            {F : Type}
+            {ar : F -> Ty B}
+            (s : Sub ar C1 C2)
+  : compSub (dropSub A s) (keepSub A (idSub C1 ar))
+    =
+    dropSub A s.
+Proof.
+  induction s ; simpl.
+  - reflexivity.
+  - rewrite IHs ; clear IHs.
+    f_equal.
+    rewrite wkTm_is_subTm.
+    rewrite subTm_comp.
+    f_equal.
+    exact (Sub_id_right (wkToSub (Drop A (idWk C1)))).
+Qed.
+
+Proposition subTm_id
+            {B : Type}
+            {C : Con B}
+            {A : Ty B}
+            {F : Type}
+            {ar : F -> Ty B}
+            (t : Tm ar C A)
+  : subTm t (idSub C ar) = t.
+Proof.
+  induction t ; simpl.
+  - reflexivity.
+  - apply subVar_id.
+  - simpl.
+    rewrite <- IHt.
+    f_equal.
+    rewrite !subTm_comp.
+    f_equal.
+    simpl ; cbn.
+    rewrite keep_drop.
+    reflexivity.
+  - rewrite IHt1, IHt2.
+    reflexivity.
+Qed.
