Code/Syntax/StrongNormalization/SN.v
@@ -1,0 +1,95 @@
+Require Import Prelude.Wellfounded.
+Require Import Syntax.Signature.
+
+Import AFSNotation.
+
+Definition isSN
+           {B F R : Type}
+           (X : AFS B F R)
+  : Prop
+  := forall (C : Con B) (A : Ty B), Wf (@Rew _ _ _ X C A).
+
+Definition Ty_isSN
+           {B F R : Type}
+           (X : AFS B F R)
+           (A : Ty B)
+  : Prop
+  := forall (C : Con B), Wf (@Rew _ _ _ X C A).
+
+Definition map_Tm
+           {B F R : Type}
+           {X : AFS B F R}
+           {C : Con B}
+           (A : Ty B)
+           {A' : Ty B}
+           (t : Tm X C A')
+  : Tm X ((A' ⟶ A),, C) A
+  := TmVar Vz · wkTm t (Drop _ (idWk C)).
+
+Definition Rew_Wk
+           {B F R : Type}
+           {X : AFS B F R}
+           {C1 C2 : Con B}
+           {A : Ty B}
+           {t1 t2 : Tm X C2 A}
+           (w : Wk C1 C2)
+           (p : Rew X t1 t2)
+  : Rew X (wkTm t1 w) (wkTm t2 w).
+Proof.
+  revert w.
+  revert C1.
+  induction p ; intros C1 w ; simpl.
+  - exact (Trans (IHp1 C1 w) (IHp2 C1 w)).
+  - exact (Rew_App_l _ (IHp C1 w)).
+  - exact (Rew_App_r _ (IHp C1 w)).
+  - exact (Rew_Lam (IHp _ (Keep A1 w))).
+  - simpl.
+    rewrite !wkTm_is_subTm.
+    rewrite subTm_comp.
+    assert (compSub
+              (wkToSub (Keep A1 w))
+              (idSub C1 (Arity X) & subTm x (wkToSub w))
+            =
+            compSub
+              (idSub C (Arity X) & x)
+              (wkToSub w)) as H.
+    {      
+      admit.
+    }
+    unfold beta_sub.
+    rewrite <- H.
+    rewrite <- subTm_comp.
+    apply Beta.
+  - rewrite !wkTm_is_subTm.
+    rewrite !subTm_comp.
+    apply BaseRew.
+Admitted.
+
+Definition Rew_map_Tm
+           {B F R : Type}
+           {X : AFS B F R}
+           {C : Con B}
+           {A A' : Ty B}
+           {t1 t2 : Tm X C A'}
+           (p : Rew X t1 t2)
+  : Rew X (map_Tm A t1) (map_Tm A t2).
+Proof.
+  unfold map_Tm.
+  apply Rew_App_r.
+  apply Rew_Wk.
+  exact p.
+Qed.
+
+Theorem SN_if_TySN
+        {B F R : Type}
+        (X : AFS B F R)
+        (A : Ty B)
+        (H : Ty_isSN X A)
+  : isSN X.
+Proof.
+  intros C A'.
+  simple refine (fiber_is_Wf (H ((A' ⟶ A) ,, C)) _ _).
+  - exact (map_Tm _).
+  - intros t1 t2.
+    exact Rew_map_Tm.
+Qed.    
